Minterop.fst
@@ -263,6 +263,7 @@ instance importable_M4_to_pi_GIO t1 t2 {| d1:exportable t1 |} {| d2:ml t2 |} :
         let tree = reify (f x) (fun r -> True) in
         _import_M4_to_GIO #t2 tree pi <: GIO t2 pi) in Some f')
 
+
 instance importable_M4_to_GIO 
   t1 {| d1:exportable t1 |} 
   t2 {| d2:ml t2 |} 
@@ -340,35 +341,94 @@ let plugin1 : file_descr -> M4 unit = fun fd ->
 // the post has to accept as a result any errors, espicially 
 // Contract_failure
 
-// let extract_local_events (s0 s1:events_trace) :
-//   Pure events_trace
-//     (requires (exists le. s1 == apply_changes s0 le))
-//     (ensures (fun le -> s1 == apply_changes s0 le)) = 
-//   admit ();
-//   assert (List.length s1 >= List.length s0);
-//   let n : nat = (List.length s1) - (List.length s0) in
-//   let (le, _) = List.Tot.Base.splitAt n s1 in
-//   List.rev le
-
-// instance importable_M4_to_IOStHist t1 t2 (post : t1 -> events_trace -> maybe (events_trace * t2) -> events_trace -> Type0)
-//   {| d1:exportable t1 |} {| d2:ml t2 |} {| checkable4 post |}:
-//   importable(x:t1 -> IOStHistwp t2 (fun s0 p -> forall res le. post x s0 res le ==>  p res le)) =
-//   mk_importable (d1.etype -> M4 t2) #(x:t1 -> IOStHistwp t2 (fun s0 p -> forall restl le. post x s0 restl le ==>  p restl le)) 
-//     (fun (f:(d1.etype -> M4 t2)) ->
-//       (fun (x:t1) ->
-//         let s0 : events_trace = IOStHist.get () in
-//         rev_append_rev_append ();
-//         let x' : d1.etype = export x in
-//         assume (forall x err s0 le. post x s0 (Inr err) le == true);
-//         let tree = reify (f x') (fun r -> True) in
-//         let result = _import_M4_to_IOStHist #t2 tree in
-//         let s1 : events_trace = IOStHist.get () in
-//         let le = extract_local_events s0 s1 in
+let extract_local_events (s0 s1:events_trace) :
+  Pure events_trace
+    (requires (exists le. s1 == apply_changes s0 le))
+    (ensures (fun le -> s1 == apply_changes s0 le)) = 
+  admit ();
+  assert (List.length s1 >= List.length s0);
+  let n : nat = (List.length s1) - (List.length s0) in
+  let (le, _) = List.Tot.Base.splitAt n s1 in
+  List.rev le
 
 
-//         // the casting is done wrongly because you don't have an extra le...
-//         // in a way this is not correct because it uses the materialized le ^ and the ghost le
-//         // without realizing that are the same thing.
-//         (if check4 #t1 #t2 #post x s0 (Inl (s1, result)) le then (admit (); result)
-//         else (IOStHist.throw Contract_failure)) ))
-//           //<: IOStHistwp t2 (fun s0 p -> forall resxy le. post x s0 resxy le ==>  p resxy le)))
+let _import_M44_to_GIO
+  (t1:Type) {| d1:exportable t1 |}
+  (t2:Type) {| d2:ml t2 |}
+  (f:(d1.etype -> M4 t2))
+  (pi:check_type) :
+  Tot (t1 -> GIO t2 pi) = admit ()
+
+let someother
+  (t1:Type) {| d1:exportable t1 |}
+  (t2:Type) {| d2:ml t2 |}
+  (post : t1 -> events_trace -> maybe (events_trace * t2) -> events_trace -> Type0) 
+  (_:squash (forall x err s0 le. post x s0 (Inr err) le == true))
+  {| d3:checkable4 post |}
+  (f:(d1.etype -> M4 t2))
+  (pi:check_type)
+  (x:t1) :
+  IOStHist t2
+    (gio_pre pi)
+    (fun h res le -> gio_post pi h res le /\ post x h res le) 
+  by (
+    explode ();
+    bump_nth 23;
+    let zz = get_binder 13 in 
+    focus (fun () ->
+      let _ = t_destruct zz in
+      iterAll (fun () ->
+        let bs = repeat intro in
+        let b = last bs in (* this one is the equality *)
+        rewrite_eqs_from_context ();
+        norm [iota];
+        ())
+    );
+    let aq = get_binder 16 in
+    focus (fun () -> 
+      let _ = t_destruct aq in
+      let bs1 = intro () in
+      let br = intro () in
+      let b = intro () in (* this one is the equality *)
+      rewrite_eqs_from_context ();
+      norm [iota];
+      let goal = match (List.Tot.Base.nth (goals ()) 0) with
+      | Some z -> z | None -> fail "Asd" in
+      let _ = inspect (goal) in
+      ()
+    );
+    dump "h"
+  ) =
+  // rev_append_rev_append ();
+  // assume (forall x err s0 le. post x s0 (Inr err) le == true);
+  let (f':t1 -> GIO t2 pi) = _import_M44_to_GIO t1 t2 f pi in
+  let s0 : events_trace = IOStHist.get () in
+  let result : t2 = f' x in
+  let s1 : events_trace = IOStHist.get () in
+  let le = extract_local_events s0 s1 in
+
+  // // the casting is done wrongly because you don't have an extra le...
+  // // in a way this is not correct because it uses the materialized le ^ and the ghost le
+  // // without realizing that are the same thing.
+  if check4 #t1 #t2 #post #d3 x s0 (Inl (s1, result)) le then (
+    assert (post x s0 (Inl (s1, result)) le);
+    result
+  ) else (
+    IOStHist.throw Contract_failure
+  )
+  
+
+
+instance importable_M4_to_IOStHist 
+  (t1:Type) {| d1:exportable t1 |}
+  (t2:Type) {| d2:ml t2 |}
+  (post : t1 -> events_trace -> maybe (events_trace * t2) -> events_trace -> Type0) 
+  {| checkable4 post |} :
+  Tot (importable (x:t1 -> IOStHistwp t2 (fun s0 p -> forall res le. post x s0 res le ==>  p res le))) =
+  mk_importable 
+    (d1.etype -> M4 t2) 
+    #(x:t1 -> IOStHistwp t2 (fun s0 p -> forall restl le. post x s0 restl le ==>  p restl le)) 
+    (fun (f:(d1.etype -> M4 t2)) -> Some (someother t1 t2 post f))
+
+
+
